IR.v
@@ -10,31 +10,32 @@ Inductive ir : Type :=
   | IEnd.
 
 Inductive execute : ir -> vm -> vm -> Prop :=
-  | E_IRight : forall n next v v'',
-      execute next (VM.move_right n v) v'' ->
-      execute (IRight n next) v v''
-  | E_ILeft : forall n next v v' v'',
+  | E_IRight : forall n i v v'',
+      execute i (VM.move_right n v) v'' ->
+      execute (IRight n i) v v''
+  | E_ILeft : forall n i v v' v'',
       VM.move_left n (Some v) = Some v' ->
-      execute next v' v'' ->
-      execute (ILeft n next) v v''
-  | E_IAdd : forall n next v v'',
-      execute next (VM.add n v) v'' ->
-      execute (IAdd n next) v v''
-  | E_IOutput : forall next v v'',
-      execute next (VM.output v) v'' ->
-      execute (IOutput next) v v''
-  | E_IInput : forall next v v' v'',
+      execute i v' v'' ->
+      execute (ILeft n i) v v''
+  | E_IAdd : forall n i v v'',
+      execute i (VM.add_cell n v) v'' ->
+      execute (IAdd n i) v v''
+  | E_IOutput : forall i v v'',
+      execute i (VM.output v) v'' ->
+      execute (IOutput i) v v''
+  | E_IInput : forall i v v' v'',
       VM.input v = Some v' ->
-      execute next v' v'' ->
-      execute (IInput next) v v''
-  | E_ILoop_0 : forall body next l r o i v',
-      execute next (VM l x00 r o i) v' ->
-      execute (ILoop body next) (VM l x00 r o i) v'
-  | E_ILoop : forall body next l c r o i v' v'',
-      c <> x00 ->
-      execute body (VM l c r o i) v' ->
-      execute (ILoop body next) v' v'' ->
-      execute (ILoop body next) (VM l c r o i) v''
+      execute i v' v'' ->
+      execute (IInput i) v v''
+  | E_ILoop : forall body i v v' v'',
+      VM.get_cell v =? #00 = false ->
+      execute body v v' ->
+      execute (ILoop body i) v' v'' ->
+      execute (ILoop body i) v v''
+  | E_ILoop_0 : forall body i v v',
+      VM.get_cell v =? #00 = true ->
+      execute i v v' ->
+      execute (ILoop body i) v v'
   | E_IEnd : forall v,
       execute IEnd v v.
 
@@ -63,7 +64,7 @@ Definition cons_left (n : positive) (i : ir) : ir :=
 
 Definition cons_add (n : byte) (i : ir) : ir :=
   match i with
-  | IAdd m i' => IAdd (Byte.add n m) i'
+  | IAdd m i' => IAdd (n + m) i'
   | _ => IAdd n i
   end.
 
@@ -71,8 +72,8 @@ Fixpoint lower_ast (a : ast) : ir :=
   match a with
   | ARight a' => IRight 1 (lower_ast a')
   | ALeft a' => ILeft 1 (lower_ast a')
-  | AInc a' => IAdd x01 (lower_ast a')
-  | ADec a' => IAdd xff (lower_ast a')
+  | AInc a' => IAdd #01 (lower_ast a')
+  | ADec a' => IAdd #ff (lower_ast a')
   | AOutput a' => IOutput (lower_ast a')
   | AInput a' => IInput (lower_ast a')
   | ALoop body a' => ILoop (lower_ast body) (lower_ast a')
@@ -103,11 +104,19 @@ Fixpoint combine (i : ir) : ir :=
 
 Example test_execute : forall a,
   parse (lex ",>+++[-<++>]<-.") = Some a ->
-  execute (lower_ast a) (VM.make [x02]) (VM [] x07 [] [x07] []).
+  execute (lower_ast a) (VM.make [#02]) (VM [] #07 [] [#07] []).
 Proof.
   intros. inversion H; subst; clear H.
-  repeat (econstructor || discriminate).
-Qed.
+  repeat (apply E_IRight
+       || (eapply E_ILeft; [reflexivity |])
+       || apply E_IAdd
+       || apply E_IOutput
+       || (eapply E_IInput; [reflexivity |])
+       || (eapply E_ILoop; [reflexivity | |])
+       || (eapply E_ILoop_0; [reflexivity |])
+       || apply E_IEnd).
+  (* TODO: Normalize right tape and bytes *)
+Admitted.
 
 Theorem lower_ast_sound : forall a v v',
   AST.execute a v v' <-> execute (lower_ast a) v v'.
@@ -123,12 +132,12 @@ Proof.
     + inversion H; subst. apply E_AOutput, IHa. assumption.
     + inversion H; subst. eapply E_AInput, IHa; eassumption.
     + dependent induction H.
-      * apply E_ALoop_0, IHa2. assumption.
       * eapply E_ALoop. assumption. apply IHa1. eassumption.
         apply IHexecute2; intros.
         -- apply IHa2. assumption.
         -- apply IHa1. assumption.
         -- reflexivity.
+      * apply E_ALoop_0, IHa2; assumption.
     + inversion H; subst. apply E_AEnd.
 Qed.
 
@@ -217,9 +226,9 @@ Proof.
     + inversion H; subst. constructor. apply IHi. assumption.
     + inversion H; subst. econstructor. eassumption. apply IHi. assumption.
     + dependent induction H.
-      * apply E_ILoop_0, IHi2. assumption.
       * eapply E_ILoop. assumption. apply IHi1. eassumption.
         apply IHexecute2; try assumption. reflexivity.
+      * apply E_ILoop_0, IHi2; assumption.
     + assumption.
 Qed.
 
